\documentclass{article}
\usepackage{amsmath}
\usepackage[total={6in, 8in}]{geometry}
\begin{document}

We want to solve:


Let $o$ be the object ball,
$p$ be the point we are solving for, 
$c$ be the source,
$d$ be the destination,
$n$ be the normal path.

We want to solve
\begin{align*}
\|p - o\| = r \\
n^T(p - o) = 0 \\
v^1 = p + t(p - s) \\
v^2 = p + s n \\
\frac 2 7 v^1 + \frac 2 5 v^2 = d \\
(v^1 - v^2)^T(v^2) = 0
\end{align*}

Let 
\begin{align*}
p \gets p - o \\
d \gets d - o \\
\end{align*}


We can let
\begin{align*}
n_0 = \pm\frac 1 r p_0 \\
n_1 = \mp\frac 1 r p_1
\end{align*}
or
so that 
\begin{align*}
n^Tp = 0 \\
n^Tn = 1
\end{align*}

We find
\begin{align*}
\|p\| = r \\
n^Tp = 0 \\
n^Tn = 1 \\
v^1 = p + t(p - c) \\
v^2 = p + s n \\
\alpha v^1 + (1 - \alpha) v^2 = p + d \\
(v^1 - v^2)^T(v^2 - p) = 0
\end{align*}

Solve for $s$:

\begin{align*}
(v^1 - v^2)^T(v^2 - p) = 0 \\
(p + t(p - c) - p - s n)^T(p + s n - p) = 0 \\
st(p - c)^Tn + s^2 n^Tn = 0 \\
t(p - c)^Tn + s = 0 \\
s = t(c - p)^Tn
\end{align*}



Plug this in:
\begin{align*}
\alpha v^1 + (1 - \alpha) v^2 = p + d \\
\alpha \left(p + t(p - c)\right) + (1 - \alpha) \left(p + s n\right) = p + d \\
\alpha t(p - c) + (1 - \alpha) s n = d \\
\alpha t(p - c) + (1 - \alpha) t(c - p)^Tn n = d \\
\end{align*}


Now we want:
\begin{align*}
\|p\| = r \\
\alpha (p - c) + (1 - \alpha) (c - p)^Tn n = \frac 1 t d \\
\end{align*}
or
\begin{align*}
p_1 = \pm \sqrt{r - p_0} \\
\alpha (p_0 - c_0) + (1 - \alpha) (c - p)^Tn n_0 = \frac 1 t d_0 \\
\alpha (p_1 - c_1) + (1 - \alpha) (c - p)^Tn n_1 = \frac 1 t d_1 \\
\end{align*}

We plug in
\begin{align*}
(c - p)^Tn = c_0 n_0 + c_1 n_1 - n_0 p_0 - n_1 p_1
\end{align*}

\begin{align*}
\alpha (p_0 - c_0) + (1 - \alpha) \left(c_0 n_0^2 + c_1 n_1 n_0 - n_0^2 p_0 - n_1 n_0 p_1\right) = \frac 1 t d_0 \\
\alpha (p_1 - c_1) + (1 - \alpha) \left(c_0 n_0n_1 + c_1 n_1n_1 - n_0n_1 p_0 - n_1^2 p_1\right) = \frac 1 t d_1 \\
\end{align*}
or
\begin{align*}
\left[\alpha (p_0 - c_0) + (1 - \alpha) \left(c_0 n_0^2 + c_1 n_1 n_0 - n_0^2 p_0 - n_1 n_0 p_1\right)\right] \frac{d_1}{d_0} = \frac 1 t d_1 \\
\alpha (p_1 - c_1) + (1 - \alpha) \left(c_0 n_0n_1 + c_1 n_1n_1 - n_0n_1 p_0 - n_1^2 p_1\right) = \frac 1 t d_1 \\
\end{align*}
so that

\begin{align*}
\left[\alpha (p_0 - c_0) + (1 - \alpha) \left(c_0 n_0^2 + c_1 n_1 n_0 - n_0^2 p_0 - n_1 n_0 p_1\right)\right] \frac{d_1}{d_0} \\
= \alpha (p_1 - c_1) + (1 - \alpha) \left(c_0 n_0n_1 + c_1 n_1^2 - n_0n_1 p_0 - n_1^2 p_1\right) \\
\end{align*}


\begin{align*}
\left[\alpha (p_0 - c_0) + (1 - \alpha) \left(n_0^2 \left(c_0 - p_0\right)  + c_1 n_0n_1 - p_1n_0 n_1\right)\right] \frac{d_1}{d_0} \\
= \alpha (p_1 - c_1) + (1 - \alpha) \left(n_1^2\left(c_1 -  p_1\right)+ c_0n_0n_1 - p_0n_0n_1\right) \\
\end{align*}

\begin{align*}
\alpha\left[\left(p_0 - c_0\right) \frac{d_1}{d_0} -p_1 + c_1\right] \\
+ (1 - \alpha) \left[
	n_0^2 \left(c_0 - p_0\right) \frac{d_1}{d_0} - n_1^2\left(c_1 -  p_1\right)
\right] \\
+ (1 - \alpha) \left[
	\left(c_1 n_0n_1 - p_1n_0 n_1\right)\frac{d_1}{d_0} - \left(c_0n_0n_1 - p_0n_0n_1\right)
\right] = 0
\end{align*}

with $\beta = \frac{d_1}{d_0}$
\begin{align*}
\alpha\left[\left(p_0 - c_0\right) \beta -p_1 + c_1\right] \\
+ (1 - \alpha) \left[
	n_0^2 \left(c_0 - p_0\right) \beta - n_1^2\left(c_1 -  p_1\right)
\right] \\
+ (1 - \alpha) \left[
	\left(c_1 n_0n_1 - p_1n_0 n_1\right)\beta - \left(c_0n_0n_1 - p_0n_0n_1\right)
\right] = 0
\end{align*}



% n_0 = \pm\frac 1 r p_0 \\
% n_1 = \mp\frac 1 r p_1

with $\beta = \frac{d_1}{d_0}$
\begin{align*}
\alpha\left[\left(p_0 - c_0\right) \beta -p_1 + c_1\right] \\
+ \frac 1 {r^2}(1 - \alpha) \left[
	 p_0^2 \left(c_0 - p_0\right) \beta -  p_1^2\left(c_1 -  p_1\right)
\right] \\
+ \frac 1 {r^2}(1 - \alpha) \left[
	\left( c_1 p_0 p_1 - p_0 p_1^2\right)\beta - \left(c_0p_0p_1 - p_0^2p_1\right)
\right] = 0
\end{align*}


\begin{align*}
\alpha\left[\left(p_0 - c_0\right) \beta -p_1 + c_1\right] \\
+ \frac 1 {r^2}(1 - \alpha) \left[
	 p_0^2 \left(c_0 - p_0\right) \beta -  p_1^2\left(c_1 -  p_1\right)
\right] \\
+ \frac 1 {r^2}(1 - \alpha) p_0p_1\left[
	\left( c_1 - p_1\right)\beta - \left(c_0 - p_0\right)
\right] = 0
\end{align*}


\begin{align*}
\alpha\left[\left(p_0 - c_0\right) \beta -p_1 + c_1\right] \\
+ \frac 1 {r^2}(1 - \alpha) \left[
	 p_0^2 \left(c_0 - p_0\right) \beta -  p_1^2\left(c_1 -  p_1\right)
\right] \\
+ \frac 1 {r^2}(1 - \alpha) p_0p_1\left[
	\left( c_1 - p_1\right)\beta - \left(c_0 - p_0\right)
\right] = 0
\end{align*}

% r - p_0
\begin{align*}
\alpha\left[\left(p_0 - c_0\right) \beta -p_1 + c_1\right] + \frac 1 {r^2}(1 - \alpha) \cdot\\
\left[
	 p_0^2 \left(c_0 - p_0\right) \beta -  p_1^2\left(c_1 -  p_1\right)
	+ p_0p_1\left[
		\left( c_1 - p_1\right)\beta - \left(c_0 - p_0\right)
	\right]
\right] = 0
\end{align*}


In sage:
\begin{verbatim}
p0, c0, c1, a, b, r = var('p0 c0 c1 a b r')
p1 = sqrt(1 - p0 ** 2)
sols = solve([
    a * ((p0 - c0) * b - p1 + c1) + 1 / r ** 2 * (1 - a) * (
            p0 ** 2 * (c0 - p0) * b - p1 ** 2 * (c1 - p1) 
            + p0 * p1 * ((c1 - p1) * b - (c0 - p0))
    ),],
    p0
)
\end{verbatim}

% \tiny
% \begin{align*}
% p_{0} = \frac{a b - {\left({\left(a - 1\right)} b c_{1} - {\left(a - 1\right)} c_{0}\right)} \sqrt{-p_{0}^{2} + 1} - \sqrt{a^{2} b^{2} + 2 \, {\left(a^{2} - 2 \, a + 1\right)} b c_{0} c_{1} - {\left(4 \, {\left(a - 1\right)} b^{2} - a^{2} + 2 \, a - 1\right)} c_{0}^{2} + {\left({\left(a^{2} - 2 \, a + 1\right)} b^{2} + 4 \, a^{2} - 4 \, a\right)} c_{1}^{2} - {\left({\left(a^{2} - 2 \, a + 1\right)} b^{2} c_{1}^{2} - 2 \, {\left(a^{2} - 2 \, a + 1\right)} b c_{0} c_{1} + {\left(a^{2} - 2 \, a + 1\right)} c_{0}^{2}\right)} p_{0}^{2} - 2 \, {\left({\left(a^{2} - a\right)} b c_{0} + {\left({\left(a^{2} - a\right)} b^{2} + 2 \, a^{2} - 2 \, a\right)} c_{1}\right)} \sqrt{-p_{0}^{2} + 1}}}{2 \, {\left({\left(a - 1\right)} b c_{0} + {\left(a - 1\right)} c_{1}\right)}}, \\
% p_{0} = \frac{a b - {\left({\left(a - 1\right)} b c_{1} - {\left(a - 1\right)} c_{0}\right)} \sqrt{-p_{0}^{2} + 1} + \sqrt{a^{2} b^{2} + 2 \, {\left(a^{2} - 2 \, a + 1\right)} b c_{0} c_{1} - {\left(4 \, {\left(a - 1\right)} b^{2} - a^{2} + 2 \, a - 1\right)} c_{0}^{2} + {\left({\left(a^{2} - 2 \, a + 1\right)} b^{2} + 4 \, a^{2} - 4 \, a\right)} c_{1}^{2} - {\left({\left(a^{2} - 2 \, a + 1\right)} b^{2} c_{1}^{2} - 2 \, {\left(a^{2} - 2 \, a + 1\right)} b c_{0} c_{1} + {\left(a^{2} - 2 \, a + 1\right)} c_{0}^{2}\right)} p_{0}^{2} - 2 \, {\left({\left(a^{2} - a\right)} b c_{0} + {\left({\left(a^{2} - a\right)} b^{2} + 2 \, a^{2} - 2 \, a\right)} c_{1}\right)} \sqrt{-p_{0}^{2} + 1}}}{2 \, {\left({\left(a - 1\right)} b c_{0} + {\left(a - 1\right)} c_{1}\right)}}
% \end{align*}




% 
% One case is
% 
% % n_0 = (\pm\frac 1 r p_0)
% % n_1 = (\mp\frac 1 r \pm \sqrt{r - p_0})
% % p_1 = (\pm \sqrt{r - p_0})
% \begin{align*}
% \left[\alpha (p_0 - c_0) + (1 - \alpha) \left(c_0 n_0^2 + c_1 n_1 n_0 - n_0^2 p_0 - n_1 n_0 p_1\right)\right] 
% \frac{d_1}{d_0} \\
% = \alpha (p_1 - c_1) + (1 - \alpha) \left(c_0 n_0n_1 + c_1 n_1^2 - n_0n_1 p_0 - n_1^2 p_1\right) \\
% \end{align*}
% 
% 
% 
% 
% \begin{align*}
% \alpha (p_0 - c_0)\frac{d_1}{d_0} + (1 - \alpha) \\
% \left(c_0 (\pm\frac 1 r p_0)^2 + c_1 (\mp\frac 1 r (\pm \sqrt{r - p_0})) (\pm\frac 1 r p_0) - (\pm\frac 1 r p_0)^2 p_0 - (\mp\frac 1 r (\pm \sqrt{r - p_0})) (\pm\frac 1 r p_0) (\pm \sqrt{r - p_0})\right)\frac{d_1}{d_0} \\
% = \alpha ((\pm \sqrt{r - p_0}) - c_1) + (1 - \alpha) \\
% \left(c_0 (\pm\frac 1 r p_0)(\mp\frac 1 r (\pm \sqrt{r - p_0})) + c_1 (\mp\frac 1 r (\pm \sqrt{r - p_0}))^2 - (\pm\frac 1 r p_0)(\mp\frac 1 r (\pm \sqrt{r - p_0})) p_0 - (\mp\frac 1 r (\pm \sqrt{r - p_0}))^2 (\pm \sqrt{r - p_0})\right) \\
% \end{align*}


\end{document}
